Add Early_accept_spec.

automata.v
@@ -77,14 +77,24 @@ revert s t; induction w as [|c w]; simpl; intros.
 Qed.
 
 Theorem Accepts_determine w s :
-  Accepts w s -> ∃t, In t s /\ Accepts w [t].
+  Accepts w s <-> ∃t, In t s /\ Accepts w [t].
 Proof.
 induction s; simpl; intros.
-- exfalso; eapply not_Accepts_nil, H.
-- replace (a :: s) with ([a] ++ s) in H by easy.
-  apply Accepts_app in H as [H|H].
-  + exists a; split. now left. easy.
-  + apply IHs in H as [t Ht]; exists t; split. now right. easy.
+- split; intros; exfalso.
+  eapply not_Accepts_nil, H. now destruct H.
+- replace (a :: s) with ([a] ++ s) by easy.
+  rewrite Accepts_app, IHs. split.
+  + intros [H|[t H]]; [exists a|exists t]; split.
+    now left. easy. now right. easy.
+  + intros [t [[R|Hs] Ht]]; subst. now left.
+    right; exists t; easy.
+Qed.
+
+Theorem Similar_accept s t :
+  Similar [s] [t] -> accept A s = accept A t.
+Proof.
+intros H; assert(H' := H []); simpl in H'.
+rewrite ?orb_false_r in H'. apply eq_iff_eq_true, H'.
 Qed.
 
 End Definitions.
@@ -425,10 +435,10 @@ Section Retraction.
 Variable A : automaton letter.
 Variable p : letter.
 
-Fixpoint retr_accept (n : nat) : state A -> bool :=
+Fixpoint retr_accept n s : bool :=
   match n with
-  | 0 => accept A
-  | S m => λ s, existsb (retr_accept m) (trans A p s)
+  | 0 => false
+  | S m => accept A s || existsb (retr_accept m) (trans A p s)
   end.
 
 (* Define early accept states using graph connectivity. *)
@@ -441,11 +451,66 @@ Hypothesis can_spec : ∀s, In (can s) Q /\ Similar A [s] [can s].
 Definition fixed_adj s := map can (trans A p s).
 Definition Early_accept := Connected fixed_adj (λ s, accept A s = true).
 
-Theorem retr_accept_spec s :
+Theorem Early_accept_spec s :
+  Early_accept Q s <-> ∃n, Accepts A (repeat p n) [s].
+Proof.
+split.
+- (* From a path to an accepted p* string. *)
+  intros [pad]; exists (path_length pad); induction pad; simpl.
+  rewrite e; easy. rewrite app_nil_r.
+  apply in_map_iff in i0 as [w' [R Hw]]; subst.
+  apply Accepts_determine; exists w'; split. easy.
+  apply can_spec, IHpad.
+- (* From an accepted p* string to a path. *)
+  intros [n H]. revert H; revert s; induction n; simpl; intros.
+  + rewrite orb_false_r in H; apply conn, path_stop, H.
+  + rewrite app_nil_r in H; apply Accepts_determine in H as [t [H1 H2]].
+    apply can_spec, IHn in H2 as [pad]. apply conn, path_step with (w:=can t).
+    apply can_spec. apply in_map, H1. apply pad.
+Qed.
+
+Lemma retr_accept_Similar s t n :
+  Similar A [s] [t] -> retr_accept n s = retr_accept n t.
+Proof.
+revert s t; induction n; simpl; intros. easy.
+rewrite Similar_accept with (t:=t). 2: apply H.
+destruct (accept A t); simpl. easy.
+apply eq_iff_eq_true; rewrite ?existsb_exists.
+split; intros [s' H'].
+(*
+There is an intuitive sense that this should hold, but the proof is not clear.
+The definition of Similar is making this much harder than it should be. I think
+I should replace Similar with a definition of isomorphic states which is defined
+directly relative to accept and trans.
+*)
+Admitted.
+
+Theorem retr_accept_Early_accept n s :
+  retr_accept n s = true -> Early_accept Q s.
+Proof.
+revert s; induction n; simpl; intros. easy. b_Prop.
+- apply conn, path_stop, e.
+- apply existsb_exists in e as [t [H1 H2]].
+  rewrite retr_accept_Similar with (t:=can t) in H2; apply IHn in H2 as [pad].
+  apply conn, path_step with (w:=can t).
+  apply can_spec. apply in_map, H1. apply pad. apply can_spec.
+Qed.
+
+Theorem Early_accept_retr_accept s :
+  Early_accept Q s -> retr_accept (length Q) s = true.
+Proof.
+Admitted.
+
+Corollary existsb_retr_accept_Accepts_repeat s :
   existsb (retr_accept (length Q)) s = true <-> ∃n, Accepts A (repeat p n) s.
 Proof.
-transitivity (Exists (Early_accept Q) s).
-Admitted.
+rewrite existsb_exists; split; intros [i H].
+- destruct H as [Hs Hi].
+  apply retr_accept_Early_accept, Early_accept_spec in Hi as [n Hi].
+  exists n; apply Accepts_determine; exists i; easy.
+- apply Accepts_determine in H as [t H]; exists t; split. easy.
+  apply Early_accept_retr_accept, Early_accept_spec. exists i; apply H.
+Qed.
 
 End Early_accept_states.
 
@@ -460,8 +525,7 @@ Proof.
 revert s; induction word as [|c w]; simpl; intros.
 - destruct finite as [Q [Q_len Hcan]].
   apply sigma_function in Hcan as [can can_spec].
-  rewrite <-Q_len, retr_accept_spec with (can:=can).
-  easy. apply can_spec.
+  rewrite <-Q_len; eapply existsb_retr_accept_Accepts_repeat, can_spec.
 - apply IHw.
 Qed.
 
@@ -517,7 +581,7 @@ Theorem Acceptable_Accepts s :
   Acceptable s -> ∃w, Accepts A w [s].
 Proof.
 intros [p]; induction p.
-- exists nil; simpl; now rewrite t.
+- exists nil; simpl; now rewrite e.
 - apply in_map_iff in i0 as [s [R Hs]]; subst.
   apply in_flat_map in Hs as [c [_ Hc]].
   destruct IHp as [w Hw].
